memcpy.v
@@ -16,13 +16,14 @@ Notation "e1 <-[ i ]{ n } ! e2" :=
   (at level 80, n, i at next level,
    format "e1  <-[ i ]{ n }  ! e2") : lrust_expr_scope.
 
-Lemma wp_memcpy `{heapG Σ} E l1 l2 vl1 vl2 q n Φ:
+Lemma wp_memcpy `{heapG Σ} E l1 l2 vl1 vl2 q n:
   nclose heapN ⊆ E →
   length vl1 = n → length vl2 = n →
-  heap_ctx ★ l1 ↦★ vl1 ★ l2 ↦★{q} vl2 ★
-  ▷ (l1 ↦★ vl2 ★ l2 ↦★{q} vl2 ={E}=★ Φ #()) ⊢ WP #l1 <-{n} !#l2 @ E {{ Φ }}.
+  {{{ heap_ctx ★ l1 ↦★ vl1 ★ l2 ↦★{q} vl2 }}}
+    #l1 <-{n} !#l2 @ E
+  {{{; #(), l1 ↦★ vl2 ★ l2 ↦★{q} vl2 }}}.
 Proof.
-  iIntros (? Hvl1 Hvl2) "(#Hinv&Hl1&Hl2&HΦ)".
+  iIntros (? Hvl1 Hvl2 Φ) "[(#Hinv & Hl1 & Hl2) HΦ]".
   iLöb as "IH" forall (n l1 l2 vl1 vl2 Hvl1 Hvl2). wp_rec. wp_op=> ?; wp_if.
   - iApply "HΦ". assert (n = O) by lia; subst.
     destruct vl1, vl2; try discriminate. by iFrame.
